case_studies/closures/ndbclo.v
@@ -14,7 +14,7 @@ From Coq Require Import List Program.Equality Unicode.Utf8.
 Import List.ListNotations.
 From Hammer Require Import Tactics.
 From VST.msl Require Import sepalg.
-From CARVe Require Import contexts.list algebras.purely_linear.
+From CARVe Require Import contexts.list algebras.linear.
 
 Ltac inv H := inversion H; subst; clear H; trivial.
 
@@ -50,13 +50,16 @@ Notation "'unit'"  := ut (in custom stlc at level 0).
 Definition tenv := lctx ty mult.
 
 Inductive has_type : tenv → tm → ty → Prop :=
-| t_Unit: forall Δ, exh hal Δ → has_type Δ <{unit}> Ty_Unit
-| t_Var: forall Δ Δ' T n,
-    updn Δ n T T one zero Δ' → exh hal Δ' → has_type Δ (var n) T
-| t_Abs: forall Δ T1 T2 t1,
-    has_type ((T2, one)::Δ) t1 T1 →
+| t_Unit {Δ} : exh _ _ hal Δ → has_type Δ <{unit}> Ty_Unit
+| t_Var {Δ Δ' T n} :
+  lookup _ _ Δ n = Some (T, one) →
+  upd _ _ Δ n (T, zero) = Δ' → 
+  exh _ _ hal Δ' →
+  has_type Δ (var n) T
+| t_Abs {Δ T1 T2 t1} :
+    has_type ((T2, one) :: Δ) t1 T1 →
     has_type Δ <{/\ t1}> (Ty_Arrow T2 T1)
-| t_App: forall Δ Δ1 Δ2 T1 T2 t1 t2,
+| t_App {Δ Δ1 Δ2 T1 T2 t1 t2} :
     has_type Δ1 t1 (Ty_Arrow T2 T1) →
     has_type Δ2 t2 T2 →
     join Δ1 Δ2 Δ →
@@ -76,13 +79,13 @@ Definition env := list val.
 
 Inductive hasty_env : env → tenv → Prop :=
 | type_empty: hasty_env nil nil
-| type_cons: forall e Δ v T m,
+| type_cons {e Δ v T m} :
     hasty_env e Δ →
     has_ty v T →
     hasty_env (v :: e) ((T, m) :: Δ)
 with has_ty : val → ty → Prop :=
 | type_unit: has_ty unit Ty_Unit
-| type_closure: forall e Δ T t1,
+| type_closure {e Δ T t1} :
     has_type Δ <{/\ t1}> T →
     hasty_env e Δ →
     has_ty (closure e <{/\ t1}>) T.
@@ -95,36 +98,27 @@ Notation "η '~' Δ" := (hasty_env η Δ) (at level 40).
 (* -------------------------------------------- *)
 
 (* If η ~ Δ and Δ₁ ⋈ Δ₂ = Δ, then η ~ Δ₁ (and Δ₂ by commutativity) *)
-Lemma merge_ctxrel_pres1: forall Δ1 Δ2 Δ η,
-    join Δ1 Δ2 Δ → hasty_env η Δ → hasty_env η Δ1.
-Proof.
-  intros.
-  generalize dependent Δ1.
-  generalize dependent Δ2.
-  induction H0; fcrush.
-Qed.
+Lemma merge_ctxrel_pres1 : ∀ Δ1 Δ2 Δ η,
+  join Δ1 Δ2 Δ → hasty_env η Δ → hasty_env η Δ1.
+Proof. intros. generalize dependent Δ1; generalize dependent Δ2; induction H0; fcrush. Qed.
 
-Lemma merge_ctxrel_pres2: forall Δ1 Δ2 Δ η,
-    join Δ1 Δ2 Δ → hasty_env η Δ → hasty_env η Δ2.
-Proof.
-  intros.
-  apply join_comm in H.
-  eapply merge_ctxrel_pres1; eassumption.
-Qed.
+Lemma merge_ctxrel_pres2 : ∀ Δ1 Δ2 Δ η,
+  join Δ1 Δ2 Δ → hasty_env η Δ → hasty_env η Δ2.
+Proof. intros. apply join_comm in H. eapply merge_ctxrel_pres1; eassumption. Qed.
 
 (* -------------------------------------------- *)
 (* Evaluation of terms                          *)
 (* -------------------------------------------- *)
 
 Inductive lookup_venv : nat → val → env → Prop :=
-| vlook_t : forall W η, lookup_venv 0 W (W :: η)
-| vlook_n : forall n W η W', lookup_venv n W η → lookup_venv (S n) W (W' :: η).
+| vlook_t : ∀ W η, lookup_venv 0 W (W :: η)
+| vlook_n {n W η} : ∀ W', lookup_venv n W η → lookup_venv (S n) W (W' :: η).
 
-Inductive eval: env → tm → val → Prop :=
-| eval_unit: forall e, eval e <{unit}> unit
-| eval_var: forall n W η, lookup_venv n W η → eval η (var n) W
-| eval_abs: forall e t1, eval e <{/\ t1}> (closure e <{/\ t1}>)
-| eval_app: forall e e' t1 t2 t3 v v',
+Inductive eval : env → tm → val → Prop :=
+| eval_unit: ∀ e, eval e <{unit}> unit
+| eval_var {n W η} : lookup_venv n W η → eval η (var n) W
+| eval_abs: ∀ e t1, eval e <{/\ t1}> (closure e <{/\ t1}>)
+| eval_app {e e' t1 t2 t3 v v'} :
     eval e t2 (closure e' <{/\ t1}>) →
     eval e t3 v' →
     eval (v' :: e') t1 v →
@@ -138,10 +132,11 @@ Notation "η '⊢' e '>>' w" := (eval η e w) (at level 40).
 
 (* Determine a value's type by performing a look-up in the linear context:
 If η ~ Δ, A¹ ∈ₙ Δ, and W ∈ₙ η, then W : A *)
-Lemma lookup_hasty: forall η n W,
-    lookup_venv n W η → forall Δ Δ' m m' A,
+Lemma lookup_hasty {η n W} :
+  lookup_venv n W η →
+  ∀ Δ m A,
     hasty_env η Δ →
-    updn Δ n A A m m' Δ' →
+    lookup _ _ Δ n = Some (A, m) →
     has_ty W A.
 Proof.
   intros * Hlookup.
@@ -154,8 +149,8 @@ Qed.
 (* Subject reduction                            *)
 (* -------------------------------------------- *)
 
-Theorem consistency : forall η M W Δ T,
-    eval η M W → hasty_env η Δ → has_type Δ M T → has_ty W T.
+Theorem consistency {η M W Δ T} :
+  eval η M W → hasty_env η Δ → has_type Δ M T → has_ty W T.
 Proof.
   intros.
   generalize dependent Δ.
@@ -190,7 +185,7 @@ Fixpoint Reduce (T : ty) (w : val) : Prop :=
   | Ty_Arrow T1 T2 =>
     match w with
     | closure η <{/\ t1}> =>
-        forall a, Reduce T1 a → exists b, eval (a :: η) t1 b ∧ Reduce T2 b
+        ∀ a, Reduce T1 a → ∃ b, eval (a :: η) t1 b ∧ Reduce T2 b
     | _ => False
     end
   end.
@@ -203,39 +198,40 @@ Notation "W ∈ T" := (Reduce T W) (at level 40).
 
 (* Semantic typing for environments *)
 Inductive REG : tenv → env → Prop :=
-| REGn: REG nil nil
-| REGc1 Δ η W A m : REG Δ η → Reduce A W →
+| REGn : REG nil nil
+| REGc1 {Δ η W A} m : REG Δ η → Reduce A W →
     REG ((A, m) :: Δ) (W :: η).
 
 Notation "Δ '~~' η" := (REG Δ η) (at level 40).
 
 (*Semantic typing for terms *)
 Definition Valid (Δ : tenv) (t : tm) (T : ty) : Prop :=
-  forall η, REG Δ η → exists a, eval η t a ∧ Reduce T a.
+  ∀ η, REG Δ η → ∃ a, eval η t a ∧ Reduce T a.
 
-Notation "Gamma '|=' t ':' T" := (Valid Gamma t T) (at level 40).
+Notation "Δ '|=' t ':' T" := (Valid Δ t T) (at level 40).
 
 Hint Unfold Valid : core.
 
-Lemma REG_preservation1: forall Δ1 Δ2 Δ,
-    join Δ1 Δ2 Δ → forall η, Δ ~~ η → Δ1 ~~ η.
+Lemma REG_preservation1 {Δ1 Δ2 Δ} :
+  join Δ1 Δ2 Δ → ∀ η, Δ ~~ η → Δ1 ~~ η.
 Proof.
-  intros * H. induction H; intros.
+  intros H. induction H; intros.
   - inv H; constructor.
   - inv H1. destruct x; constructor. now eapply IHlist_join. inv H0; sauto.
 Qed.
  
-Lemma REG_preservation2: forall Δ1 Δ2 Δ η,
-    join Δ1 Δ2 Δ → Δ ~~ η → Δ2 ~~ η.
+Lemma REG_preservation2 {Δ1 Δ2 Δ} η :
+  join Δ1 Δ2 Δ → Δ ~~ η → Δ2 ~~ η.
 Proof.
   intros. apply join_comm in H. eapply REG_preservation1; eassumption.
 Qed.
 
-Lemma REG_lookup: forall Δ η,
-    Δ ~~ η → forall Δ' n m m' T, updn Δ n T T m m' Δ' →
-    exists W, lookup_venv n W η ∧ W ∈ T.
+Lemma REG_lookup {Δ η} :
+  Δ ~~ η →
+  ∀ n m T, lookup _ _ Δ n = Some (T, m) →
+  ∃ W, lookup_venv n W η ∧ W ∈ T.
 Proof.
-  intros * RR. induction RR.
+  intros RR. induction RR.
   - sauto. (* impossible cases *)
   - intros * U. dependent destruction U; sauto lq: on.
 Qed.
@@ -245,14 +241,13 @@ Qed.
 (* -------------------------------------------- *)
 
 (* Well-typed terms are semantically typed *)
-Lemma fundamental: forall Δ t T, has_type Δ t T → Valid Δ t T.
+Lemma fundamental {Δ t T} : has_type Δ t T → Valid Δ t T.
 Proof.
-  unfold Valid.
-  intros Δ t ? H. induction H; intros η Rel.
+  unfold Valid. intro H. induction H; intros η Rel.
   - (* unit *) eexists; split; econstructor.
   - (* var *) 
     eapply REG_lookup in Rel.
-    destruct Rel. 2:eassumption.
+    destruct Rel. 2: eassumption.
     exists x. split.
     + constructor. firstorder. 
     + tauto.
@@ -261,20 +256,17 @@ Proof.
     split.
     + eauto using eval.
     + simpl. intros. specialize (IHhas_type (cons a η)).
-      assert ((cons (T2,one) Δ) ~~ (cons a η)) by eauto using REG.
+      assert ((cons (T2, one) Δ) ~~ (cons a η)) by eauto using REG.
       firstorder.
   - (* app *)
     assert (Rel' := Rel). assert (H1' := H1).
     assert (join Δ1 Δ2 Δ → Δ ~~ η → Δ1 ~~ η) by sfirstorder use: REG_preservation1.
-    apply H2 in H1'. clear H2.
-    apply (REG_preservation2 Δ1 Δ2 Δ η) in H1.
-    apply IHhas_type1 in H1'.
-    apply IHhas_type2 in H1.
-    2:assumption. 2:assumption.
+    apply H2, IHhas_type1 in H1'.
+    apply (REG_preservation2 η), IHhas_type2 in H1.
+    2: assumption. 2: assumption.
     sintuition.
-    destruct a; try tauto.
-    destruct t; try tauto.
-    apply (H4 a0) in H5. sintuition.
+    destruct a; try tauto. destruct t; try tauto.
+    apply (H5 a0) in H6. sintuition.
     exists b; eauto using eval.
 Qed.
 
@@ -283,8 +275,10 @@ Qed.
 (* -------------------------------------------- *)
 
 (* Totality of evaluation: the evaluation of any (well-typed) term is well-defined *)
-Corollary total : forall t T,
-  has_type [] t T → exists a, eval [] t a.
+Corollary total {t T} :
+  has_type [] t T →
+  ∃ a, eval [] t a.
 Proof.
-  intros. apply fundamental in H. unfold Valid in H. destruct (H nil); sfirstorder.
+  intro. apply fundamental in H. unfold Valid in H.
+  destruct (H nil); sfirstorder.
 Qed.
