case_studies/llc/progress.v
@@ -1,0 +1,37 @@
+(* ======================================================= *)
+(* Typing, context morphism lemmas, and preservation       *)
+(* (contexts as total maps)                                *)
+(* ======================================================= *)
+
+(* Imports *)
+From Coq Require Import Logic.FunctionalExtensionality Unicode.Utf8.
+From Hammer Require Import Tactics.
+From CARVe Require Import contexts.total_fun algebras.linear.
+From Autosubst Require Import fintype stlc step.
+Require Import tenv typing.
+
+(* ------------------------------------- *)
+(* Canonical forms lemma                 *)
+(* ------------------------------------- *)
+
+Lemma canonical_forms_fun : ∀ (M : tm 0) T1 T2,
+  has_type emptyT M (Fun T1 T2) →
+  value M →
+  ∃ N U, M = lam U N.
+Proof. sauto lq: on. Qed.
+
+(* ------------------------------------- *)
+(* Theorem                               *)
+(* ------------------------------------- *)
+
+(** Progress *)
+
+Lemma progress (M : tm 0) : ∀ T,
+  has_type emptyT M T →
+  value M ∨ ∃ M', step M M'.
+Proof.
+  dependent induction M; intros; try sfirstorder.
+  - right. inversion H; subst.
+    apply join_emptyT in H5; sintuition.
+    sauto use: (IHM1 M1 eq_refl JMeq_refl (Fun T2 T) H2), canonical_forms_fun.
+Qed.
